Java/src/Logic/Decidable.v
@@ -1,0 +1,145 @@
+Require Import Program  Heap ProtocolLogic AssertionLogic OperationalSemantics SpecLogic Util.
+Require Import MapInterface MapFacts.
+Require Import SepAlg SepAlgInsts ILInsts ILogic ILEmbed ILEmbedTac ILQuantTac OpenILogic
+               SepAlgMap UUSepAlg Open Subst Stack Lang SemCmd HeapArr ST SemCmdRules BILogic BILInsts Rel.
+
+
+Local Transparent ILPre_Ops.
+Local Transparent ILPreFrm_pred.
+Local Transparent EmbedSasnPureOp.
+Local Transparent EmbedILFunOp.
+Local Transparent EmbedAsnPropOp.
+Local Transparent ILPre_Ops.
+Local Transparent EmbedILPreDropOp.
+Local Transparent EmbedILPreOp.
+Local Transparent MapSepAlgOps.
+Local Transparent ILFun_Ops.
+Local Transparent EmbedILFunDropOp.
+Local Transparent EmbedILFunOp.
+Local Transparent SepAlgOps_prod.
+
+Local Transparent EmbedILPreDropOp.
+Local Transparent EmbedILFunDropOp.
+Local Transparent EmbedPSasnPropOp.
+Local Transparent EmbedAsnPropOp.
+Local Transparent BILOperatorsPSasn.
+Local Transparent BILFun_Ops.
+Local Transparent BILOperatorsAsn.
+Local Transparent ILOpsSAsn.
+
+Local Existing Instance DecSval.
+
+Lemma pointsto_decidable (v : var) (f : field) (e : expr) :
+  (* @lentails sasn _ (@ltrue sasn _) *) (DecidableAsn (`pointsto v/V `f e)).
+Proof.
+  intros (*_ _ _ _ _*) s Pr n h.
+  destruct (dec_eq (s v) null) as [Hnull | Hnotnull]; [
+    unfold var_expr; simpl; right; intro Hfail; destruct Hfail as [Hfail _]; rewrite Hnull in Hfail; auto |].
+  remember (s v) as ptr; destruct ptr;
+    try (unfold var_expr; simpl; right; intro Hfail; destruct Hfail as [Hfail _]; rewrite <- Heqptr in Hfail; apply Hfail; reflexivity).
+  assert (p <> pnull) as Hnotpnull by (intro Hfail; apply Hnotnull; unfold null; rewrite Hfail; reflexivity).
+  unfold liftn, lift, var_expr; simpl.
+  rewrite <- Heqptr in *; simpl.
+  destruct (In_dec (get_heap_ptr h) (p, f)) as [Hin | Hnotin].
+  destruct Hin as [k Hmapsto].
+  destruct (dec_eq k (e s)) as [Heq | Hneq]; [ subst |].
+  - left; split; [assumption |].
+    exists (remove (p, f) (get_heap_ptr h)).
+    apply sa_mul_swapL; [apply sa_mulC; apply uusa_unit; apply empty_1 | assumption].
+  - right. intro Hfail; destruct Hfail as [_ Hfail].
+    apply Hneq.
+    destruct Hfail as [? Hfail].
+    eapply sa_mul_mapstoR in Hfail; [| apply Hmapsto].
+    destruct Hfail as [[Hfail _] | [_ Hfail]].
+    + apply find_mapsto_iff in Hfail. rewrite add_eq_o in Hfail; [| reflexivity].
+      inversion Hfail; reflexivity.
+    + exfalso; apply Hfail; exists (e s).
+      apply add_1; reflexivity.
+  - right. intros Hfail; destruct Hfail as [_ Hfail].
+    apply Hnotin.
+    unfold subheap in Hfail; destruct Hfail as [? Hfail].
+    exists (e s).
+    eapply sa_mul_mapstoL; [apply Hfail |].
+    apply add_1; reflexivity.
+Qed.
+
+Lemma pointsto_decidable_2 (v : var) (f : field) (e : expr) (Q : sasn) :
+  DecidableAsn Q -> DecidableAsn (Q ** `pointsto v/V `f e).
+Proof.
+  unfold DecidableAsn; simpl.
+  intros (* _ _ _ _ *) H s Pr n h.
+  
+  destruct (dec_eq (s v) null) as [Hnull | Hnotnull]; [
+    unfold var_expr; right; intro Hfail; destruct Hfail as [h1 [h2 [Hh [_ [HP _]]]]]; simpl in HP; rewrite Hnull in HP; auto |].
+  remember (s v) as ptr; destruct ptr;
+    try (unfold var_expr; right; intro Hfail; destruct Hfail as [h1 [h2 [Hh [_ [HP _]]]]]; simpl in HP; rewrite <- Heqptr in HP; apply HP; reflexivity).
+  assert (p <> pnull) as Hnotpnull by (intro Hfail; apply Hnotnull; unfold null; rewrite Hfail; reflexivity).
+  
+  specialize (H s Pr n (mkheap (remove (p, f) (get_heap_ptr h)) (get_heap_arr h))).
+  destruct H as [HQ | notHQ].
+  * destruct (In_dec (get_heap_ptr h) (p, f)) as [Hin | Hnotin].
+    destruct Hin as [k Hmapsto]. 
+    destruct (dec_eq k (e s)) as [Heq | Hneq]; [ subst |].
+    - left.
+      exists (mkheap (remove (p, f) (get_heap_ptr h)) (get_heap_arr h)).
+      exists (mkheap (add (p, f) (e s) (empty _)) (empty _)).
+      assert (sa_mul (mkheap (remove (p, f) (get_heap_ptr h)) (get_heap_arr h)) 
+                     (mkheap (add (p, f) (e s) (empty val)) (empty val)) h) by (
+        apply split_heap; simpl; [apply sa_mulC; apply sa_mul_swapL; [apply sa_mulC; apply uusa_unit; apply empty_1 | apply Hmapsto] |
+      	  						  apply uusa_unit; apply empty_1]).
+      exists H.
+      split; [ apply HQ |].
+      unfold liftn, lift, var_expr; simpl.
+      rewrite <- Heqptr; simpl. split; [ apply Hnotpnull |].
+      exists (empty _); apply uusa_unit; apply empty_1.
+    - right; intro Hfail. destruct Hfail as [h1 [h2 [Hh [_ [_ HP]]]]].
+      unfold liftn, lift, var_expr in HP; simpl in HP.
+      destruct HP as [? HP].
+      rewrite <- Heqptr in HP; simpl in HP.
+      eapply sa_mul_mapstoL in HP; [| apply add_1; reflexivity ].
+      apply sa_mulC in Hh. apply isolate_heap_ptr in Hh. eapply sa_mul_mapstoL in Hh; [| apply HP].
+      destruct Hh as [Hh _].
+      apply find_mapsto_iff in Hh; apply find_mapsto_iff in Hmapsto.
+      rewrite Hh in Hmapsto.
+      apply Hneq; inversion Hmapsto; reflexivity.
+    - right. intro Hfail. destruct Hfail as [h1 [h2 [Hh [_ [_ HP]]]]].
+      unfold liftn, lift, var_expr in HP; simpl in HP.
+      apply Hnotin; exists (e s).
+      destruct HP as [? HP].
+      rewrite <- Heqptr in HP; simpl in HP.
+      eapply sa_mul_mapstoL in HP; [| apply add_1; reflexivity ].
+      apply sa_mulC in Hh. apply isolate_heap_ptr in Hh. eapply sa_mul_mapstoL in Hh; [| apply HP].
+      apply Hh.
+  * right.
+    intro Hfail; apply notHQ.
+    destruct Hfail as [h1 [h2 [Hh [HQ HP]]]].
+	solve_model HQ; unfold rel.
+	exists (mkheap (remove (p, f) (get_heap_ptr h2)) (get_heap_arr h2)).
+	apply split_heap; simpl; [| apply Hh].
+	assert (~ In (p, f) (get_heap_ptr h1)). {
+	  intro Hfail.
+	  unfold liftn, lift, var_expr in HP; simpl in HP.
+	  destruct HP as [_ [? HP]].
+	  rewrite <- Heqptr in HP; simpl in HP.
+	  eapply sa_mul_mapstoL in HP; [| apply add_1; reflexivity ].
+	  apply isolate_heap_ptr in Hh; apply sa_mulC in Hh; eapply sa_mul_inL in Hh; [| exists (e s); apply HP].
+	  destruct Hh as [Hh _].
+	  apply Hh; apply Hfail.
+    }
+    apply sa_mulC.
+    eapply sa_mul_remove; [ apply sa_mulC; apply Hh | apply H ].
+Qed.
+
+Lemma exists_decidable {A : Type} (P : A -> sasn) (a : A) : DecidableAsn( P a ) -> DecidableAsn( Exists a, P a). 
+Proof.
+  intro H.
+  intros s Pr n h.
+  specialize (H s Pr n h).
+  destruct H as [H | notH].
+  left.
+  exists a; assumption.
+  right.
+  intro Hfail.
+  destruct Hfail as [? Hfail].
+  admit.
+Admitted.  
